Test/LoweringSyntaxImport.lean
@@ -1,0 +1,11 @@
+import Crush
+
+namespace LoweringSyntaxImported
+
+def increment (x : Int) : Int := x + 1
+
+register_lowering term <<
+  (increment (term x)) => (smt| (+ $x 1))
+>>
+
+end LoweringSyntaxImported
